|\textbf{Initial and goal states}| |\vspace{5pt}|
C1. $(Q_0= q_{\mathtt{Init}}) \land (\goal(Q_n) = \true)$ |\vspace{5pt}|
|\textbf{Operator activation}| |\vspace{5pt}|
C2. $\bigwedge_{i = 0}^{n-1} \bigwedge_{F_k \subseteq F} (\sum_{p_i^o \in (P^J_i \cup  P^{F_k}_i)} p_i^o = 1)$ |\vspace{5pt}|
|\textbf{Jump constraint}| |\vspace{5pt}|
C3. $\bigwedge_{i = 0}^{n-1} \bigwedge_{j \subseteq J}  ((p^j_i = 1) \implies \texttt{cond}_j(V_i))$ |\vspace{5pt}|
C4. $\bigwedge_{i = 1}^{n} \bigwedge_{j \subseteq J}  ((p^j_i = 1) \implies (Q_i = \texttt{eff}_j(V_{i-1})))$ |\vspace{5pt}|
C5. $\bigwedge_{i = 0}^{n-1} \bigwedge_{j \in J}  ((p^j_i = 1) \implies (d_i = 0))$|\vspace{5pt}|
|\textbf{Flow constraint}| |\vspace{5pt}|
C6. $\bigwedge_{i = 0}^{n-1} \bigwedge_{f \subseteq F} (p_i^f = 1) \implies (\bigwedge_r \bigvee_s (\textit{cond}^Q_{f,rs} (Q_{i}) \land \textit{cond}^Q_{f,rs} (Q_{i+1}))) $|\vspace{5pt}|
C7. $\bigwedge_{i = 0}^{n-1} \bigwedge_{f \subseteq F} (p_i^f = 1) \implies \textit{cond}^E_{f} (E_{i})  $ |\vspace{5pt}|
C8. $\bigwedge_{i = 0}^{n-1} \bigwedge_{f \subseteq F} (p_i^f = 1) \implies \textit{cond}^\Delta_{f} (\Delta_{i}, d_i)  $ |\vspace{5pt}|
C9. $\bigwedge_{i = 0}^{n-1} \bigwedge_{f \subseteq F} ((p^f_i=1) \implies (X_{k(i+1)} - X_{ki} = A_f \Delta_i - B_fd_i))$ |\vspace{5pt}|
C10. $\bigwedge_{i = 0}^{n-1} \bigwedge_{f \in F}  ((p_i^F = 1) \implies (L_{i+1} = L_i))$|\vspace{5pt}|



